Eisbach_WP: Cleaned up with a few comments. Added another safety condition for lifting in wpstr, as well as an override for forcing postconditions through despite being apparently unsafe.

lib/wp/Eisbach_WP.thy
@@ -6,8 +6,183 @@
 
 theory Eisbach_WP
 imports "../Eisbach_Methods" NonDetMonadVCG "../Conjuncts" "../Rule_By_Method"
+        
 begin
 
+text \<open>Strengthening postconditions automatically using wp\<close>
+
+text \<open>TODO: Handle quantifiers in the post condition\<close>
+
+context begin
+
+
+text \<open>A small wrapper around implication so we can track assumptions we've added.\<close>
+
+
+definition "strong_post P Q \<equiv> P \<longrightarrow> Q"
+
+lemmas strong_post_cong = imp_cong[simplified strong_post_def[symmetric]]
+
+text \<open>A small utility method which succeeds only when two given terms share free variables.\<close>
+
+ML \<open>
+  fun has_shared_frees t t' =
+  let
+    val frees = Term.add_frees t [];
+    val frees' = Term.add_frees t' [];
+  in
+   exists (member (op =) frees') frees
+  end
+\<close>
+
+method_setup shared_frees =
+  \<open>Args.term -- Args.term >> 
+    (fn (t,t') => (fn _ =>
+    SIMPLE_METHOD (
+      if has_shared_frees t t' then all_tac else no_tac)))\<close>
+
+
+text \<open>Our counterpart to hoare_add_post.\<close>
+
+lemma hoare_strong_post:
+  "\<lbrace>P'\<rbrace> f \<lbrace>Q\<rbrace> \<Longrightarrow> 
+  \<lbrace>P''\<rbrace> f \<lbrace>\<lambda>r s. strong_post (Q r s) (H r s)\<rbrace> \<Longrightarrow> \<lbrace>\<lambda>s. P' s \<and> P'' s\<rbrace> f \<lbrace>\<lambda>r s. H r s\<rbrace>"
+  by (fastforce simp add: valid_def strong_post_def)
+
+text \<open>Similar for hoare_drop_imps. Note we can repeatedly apply this without clobbering
+      the original post condition.\<close>
+
+private lemma drop_strong_post:
+  "\<lbrace>P\<rbrace> f \<lbrace>R\<rbrace> \<Longrightarrow> \<lbrace>P\<rbrace> f \<lbrace>\<lambda>r s. strong_post (Q r s) (R r s)\<rbrace>"
+  apply (erule hoare_strengthen_post)
+  by (simp add: strong_post_def)
+
+
+text \<open>Simple test for if a function uses its first argument. This method will fail if
+      handed a post condition which ignores the return value.\<close>
+
+method uses_arg for C :: "'a \<Rightarrow> 'b \<Rightarrow> bool" =
+  (match (C) in "\<lambda>r s. ?discard_r s" (cut) \<Rightarrow> \<open>fail\<close> \<bar> _ \<Rightarrow> \<open>-\<close>)
+
+text \<open>Here "f" is the function with its arguments, C is the logical context of the post condition,
+      built up as we peel off implications, and Q is the postcondition we are decomposing
+      (and assumed to be atomic in the final match case).
+      
+      We decompose the postcondition, and assume its atomic parts given that we know how to 
+      solve them in isolation. wp_weak tries to solve the generated triple regardless, while
+      wp_strong is only applied given some safety checks on the logical context.\<close>
+
+method find_context for f :: 'd  and C Q :: "'a \<Rightarrow> 'b \<Rightarrow> bool"  methods wp_weak wp_strong =
+  (match (Q) in 
+    "\<lambda>r s. Q' r s \<and> Q'' r s" (cut) for Q' Q'' :: "'a \<Rightarrow> 'b \<Rightarrow> bool" \<Rightarrow>
+       \<open>find_context f C Q' \<open>wp_weak\<close> \<open>wp_strong\<close> , find_context f C Q'' \<open>wp_weak\<close> \<open>wp_strong\<close> \<close>
+  \<bar> "\<lambda>r s. Q' r s \<longrightarrow> Q'' r s" (cut)  for Q' Q'' :: "'a \<Rightarrow> 'b \<Rightarrow> bool" \<Rightarrow>
+       \<open>find_context f "\<lambda>r s. C r s \<and> Q' r s" Q'' \<open>wp_weak\<close> \<open>wp_strong\<close> \<close>
+  \<bar> "\<lambda>r s. if A r s then Q' r s else Q'' r s" (cut) for A Q' Q'' :: "'a \<Rightarrow> 'b \<Rightarrow> bool" \<Rightarrow>
+       \<open>find_context f "\<lambda>r s. C r s \<and> A r s" Q' \<open>wp_weak\<close> \<open>wp_strong\<close> , find_context f "\<lambda>r s. C r s \<and> \<not> A r s"  Q''\<open>wp_weak\<close> \<open>wp_strong\<close>\<close>
+  \<bar> "\<lambda>r s. Q' r s \<or> Q'' r s" (cut) for Q' Q'' :: "'a \<Rightarrow> 'b \<Rightarrow> bool" \<Rightarrow>
+       \<open>find_context f "\<lambda>r s. C r s \<and> (\<not> Q'' r s)" Q' \<open>wp_weak\<close> \<open>wp_strong\<close> , find_context f "\<lambda>r s. C r s \<and> (\<not> Q' r s)" Q'' \<open>wp_weak\<close> \<open>wp_strong\<close> \<close>
+  \<bar> "\<lambda>r. Q' r and Q'' r" (cut)  for Q' Q'' :: "'a \<Rightarrow> 'b \<Rightarrow> bool" \<Rightarrow>
+       \<open>find_context f C Q' \<open>wp_weak\<close> \<open>wp_strong\<close> , find_context f C Q'' \<open>wp_weak\<close> \<open>wp_strong\<close>\<close>    
+     
+       
+  \<bar> _ \<Rightarrow> 
+  \<open>(rule hoare_strong_post[where Q=Q], (* see if we know how to prove Q *)
+   (solves \<open>wp_weak\<close> (* try our more specific solver first (wp only: ...) *)
+   |(match (C) in "\<lambda>_ _. True" \<Rightarrow> \<open>succeed\<close> (* optimization: without context lifting is always safe *)
+    \<bar> _ \<Rightarrow> \<open>fails \<open>
+            shared_frees C Q (* consequent shares variables with antecedent *) 
+          | shared_frees f C, shared_frees f Q (* both consequent and antecedent share variables with function args *)
+          | uses_arg C, uses_arg Q (* consequent and antecedent depend on return value *)
+          | uses_arg C, shared_frees f Q (* antecedent depends on return value, consequent depends on function args *)
+          | shared_frees f C, uses_arg Q (* consequent depends on return value, antecedent depends on function args *) 
+          \<close>\<close>),  
+    solves \<open>wp_strong\<close> (* if we can assume that we don't actually depend on our logical context, try the real solver (wp) *)
+    ))?\<close>
+   )
+
+
+text \<open>After matching the conclusion we are now focused and can't affect the schematic precondition.
+      To work around this, we replace the precondition with a schematic that we can resolve after
+      focusing.\<close>
+
+definition "schematic_equiv P P' \<equiv> (P \<equiv> P')" 
+
+lemma
+  hoare_pre_schematic_equiv: 
+  "\<lbrace>Q\<rbrace> a \<lbrace>R\<rbrace> \<Longrightarrow> (\<And>s. PROP schematic_equiv (Q s) (P s))\<Longrightarrow> \<lbrace>P\<rbrace> a \<lbrace>R\<rbrace>"
+  by (simp add: schematic_equiv_def valid_def)
+  
+
+lemma schematic_equivI: "PROP schematic_equiv P P" 
+  by (simp add: schematic_equiv_def)
+ 
+
+text \<open>We focus, schematic-ify the precondition, 
+      then we enrich the postcondition. We then simplify it
+      (with our own congruence rule) and then drop our enriched postconditions.
+
+      Note that ";" limits us to the first subgoal, so defer_tac only pushes our generated
+      subgoal down by 1, leaving us with the original hoare triple after solving it with  
+      schematic_equivI.
+\<close>
+
+
+method post_strengthen methods wp_weak wp_strong simp' =
+  (match conclusion in "\<lbrace>_\<rbrace> f \<lbrace>Q\<rbrace>" for Q f \<Rightarrow>
+    \<open>rule hoare_pre_schematic_equiv, find_context f "\<lambda>_ _. True" Q \<open>wp_weak\<close> \<open>wp_strong\<close>\<close>, 
+   defer_tac, rule schematic_equivI,
+   simp'; 
+    ((rule drop_strong_post)+)
+  )
+
+named_theorems wpstr
+
+method wpstr uses add del declares wpstr = 
+  (post_strengthen \<open>wp only: wpstr\<close> \<open>wp add: add del: del\<close> \<open>simp split del: split_if cong: strong_post_cong\<close>)
+
+end
+
+notepad begin
+  fix P P' P'' P''' and Q Q' Q'' :: "'a \<Rightarrow> bool" and R :: "bool \<Rightarrow> 'b \<Rightarrow> 'a \<Rightarrow> bool"
+      and f :: "'x \<Rightarrow> ('a,'b) nondet_monad" and D D' D'' D''' D'''' y and x :: 'x
+  assume    A[wp]: "\<lbrace>P'\<rbrace> f x \<lbrace>\<lambda>_. Q\<rbrace>" and 
+            B[wp]:"\<lbrace>P''\<rbrace> f x \<lbrace>\<lambda>_. Q'\<rbrace>" and
+            C: "\<And>r s.
+                (R D r s \<longrightarrow>
+                 D \<and>
+                 (y x \<longrightarrow> D''' y) \<and> (D'''' \<longrightarrow> y x)) \<and>
+                (\<not> R D r s \<longrightarrow> Q'' s)"
+  have "\<lbrace>P and P' and P'' and (\<lambda>_. D'' x \<and> D' x)\<rbrace> 
+          f x 
+        \<lbrace>\<lambda>r s. D'' x \<and> (R D r s \<longrightarrow> (Q s \<and> Q' s \<and> D \<and> (y x \<longrightarrow> D''' y) \<and> (D''''  \<longrightarrow> y x))) \<and> 
+                (\<not> R D r s \<longrightarrow> (Q s \<and> Q'' s))\<rbrace>"
+  apply (rule hoare_pre)
+  apply wpstr
+  apply (rule hoare_strengthen_post[OF hoare_post_taut[where P=\<top>]])
+  apply (rule C)
+  by simp
+
+  fix B
+  assume B[wp]: "\<lbrace>\<lambda>s. B x s\<rbrace> f x \<lbrace>\<lambda>r s. B x s\<rbrace>"
+
+  have "\<lbrace>B x\<rbrace> f x \<lbrace>\<lambda>r s. R D r s \<longrightarrow> B x s\<rbrace>"
+  apply (rule hoare_pre)
+  apply (wpstr wpstr: B)
+  apply wp
+  by simp
+ 
+
+end
+
+
+text \<open> 
+  Methods for manipulating the post conditions of hoare triples as if they
+  were proper subgoals. I'm not convinced they are actually that useful anymore,
+  as the wpstr method mostly subsumes my intended use for them. 
+
+\<close>
+context begin
 
 definition "packed_valid P f si r s \<equiv> P si \<and> (r, s) \<in> fst (f si)"
 
@@ -77,6 +252,14 @@ method post_strong methods m_distinct m_all =
 
 method post methods m = post_strong \<open>(assumption | erule mp)+\<close> \<open>m\<close>
 
+end
+
+
+text \<open>
+  Method (meant to be used with @ as an attribute) used for producing multiple facts out of 
+  a single hoare triple with a conjunction in its post condition.
+\<close>
+
 context begin
 
 private lemma hoare_decompose: 
@@ -144,85 +327,7 @@ notepad begin
 
 end
 
-text \<open>Strengthening postconditions automatically\<close>
 
-context begin
-
-
-definition "strong_post P Q \<equiv> P \<longrightarrow> Q"
-
-
-lemmas strong_post_cong[cong] = imp_cong[simplified strong_post_def[symmetric]]
-
-
-lemma hoare_strong_post:
-  "\<lbrace>P\<rbrace> f \<lbrace>Q\<rbrace> \<Longrightarrow>
-  \<lbrace>P'\<rbrace> f \<lbrace>\<lambda>r s. strong_post (Q r s) (H r s)\<rbrace> \<Longrightarrow> \<lbrace>\<lambda>s. P s \<and> P' s\<rbrace> f \<lbrace>\<lambda>r s. H r s\<rbrace>"
-  apply (auto simp add: valid_def strong_post_def)
-  by fastforce
-
-private lemma drop_strong_post:
-  "\<lbrace>P\<rbrace> f \<lbrace>R\<rbrace> \<Longrightarrow> \<lbrace>P\<rbrace> f \<lbrace>\<lambda>r s. strong_post (Q r s) (R r s)\<rbrace>"
-  apply (erule hoare_strengthen_post)
-  by (simp add: strong_post_def)
-
-
-method find_context for Q :: "'a \<Rightarrow> 'b \<Rightarrow> bool" methods m =
-  (match (Q) in 
-    "\<lambda>r s. Q' r s \<and> Q'' r s" (cut) for Q' Q'' :: "'a \<Rightarrow> 'b \<Rightarrow> bool" \<Rightarrow>
-       \<open>find_context Q' \<open>m\<close>, find_context Q'' \<open>m\<close>\<close>
-  \<bar> "\<lambda>r s. _ \<longrightarrow> Q'' r s" (cut)  for Q'' :: "'a \<Rightarrow> 'b \<Rightarrow> bool" \<Rightarrow>
-       \<open>find_context Q'' \<open>m\<close>\<close>
-  \<bar> "\<lambda>r s. if _ then Q' r s else Q'' r s" (cut) for Q' Q'' :: "'a \<Rightarrow> 'b \<Rightarrow> bool" \<Rightarrow>
-       \<open>find_context Q' \<open>m\<close>, find_context Q'' \<open>m\<close>\<close>
-  \<bar> "\<lambda>r s. Q' r s \<or> Q'' r s" (cut) for Q' Q'' :: "'a \<Rightarrow> 'b \<Rightarrow> bool" \<Rightarrow>
-       \<open>find_context Q' \<open>m\<close>, find_context Q'' \<open>m\<close>\<close>
-  \<bar> "\<lambda>r. Q' r and Q'' r" (cut)  for Q' Q'' :: "'a \<Rightarrow> 'b \<Rightarrow> bool" \<Rightarrow>
-       \<open>find_context Q' \<open>m\<close>, find_context Q'' \<open>m\<close>\<close>
-  \<bar> _ \<Rightarrow> \<open>(rule hoare_strong_post[where Q=Q], solves \<open>m\<close>)?\<close>
-   )
-
-definition "schematic_equiv P P' \<equiv> (PROP P \<equiv> PROP P')" 
-
-lemma
-  hoare_pre_schematic_equiv: 
-  "\<lbrace>Q\<rbrace> a \<lbrace>R\<rbrace> \<Longrightarrow> (\<And>s. PROP schematic_equiv (Trueprop (Q s)) (Trueprop (P s)))\<Longrightarrow> \<lbrace>P\<rbrace> a \<lbrace>R\<rbrace>"
-  apply (simp add: schematic_equiv_def)
-  apply (rule hoare_pre_imp[rotated],assumption)
-  apply (drule_tac x=s in meta_spec)
-  by (erule equal_elim_rule2)
-  
-
-lemma schematic_equivI: "PROP schematic_equiv (PROP P) (PROP P)" 
-  by (simp add: schematic_equiv_def)
- 
-
-method post_strengthen methods wp' simp' =
-  (match conclusion in "\<lbrace>_\<rbrace> _ \<lbrace>Q\<rbrace>" for Q \<Rightarrow>
-    \<open>rule hoare_pre_schematic_equiv, find_context Q \<open>wp'\<close>\<close>, 
-   find_goal \<open>rule schematic_equivI\<close>,
-   simp'; ((rule drop_strong_post)+)?,
-   (rule hoare_vcg_prop)?
-  )
-
-
-method wpstr uses add del = 
-  (post_strengthen \<open>wp add: add del: del\<close> \<open>simp split del: split_if\<close>)
-
-end
-
-notepad begin
-  fix P P' P'' and Q Q' Q'' R :: "'b \<Rightarrow> 'a \<Rightarrow> bool" and f :: "('a,'b) nondet_monad"
-  assume A: "\<lbrace>P'\<rbrace> f \<lbrace>Q\<rbrace>" and B[wp]:"\<lbrace>P''\<rbrace> f \<lbrace>Q'\<rbrace>" and C: "\<And>r s. \<not> R r s \<longrightarrow> Q'' r s"
-  have "\<lbrace>P and P' and P''\<rbrace> f \<lbrace>\<lambda>r s. (R r s \<longrightarrow> (Q r s \<and> Q' r s)) \<and> (\<not> R r s \<longrightarrow> (Q r s \<and> Q'' r s))\<rbrace>"
-  apply (rule hoare_pre)
-   apply (wpstr add: A del: B)
-   apply wpstr
-   apply (simp add: C)
-   apply wp
-  by simp
-
-end
 
 
 end
